<?xml version="1.0"?>


<!DOCTYPE rdf:RDF [
    <!ENTITY dcterms "http://purl.org/dc/terms/" >
    <!ENTITY owl "http://www.w3.org/2002/07/owl#" >
    <!ENTITY xsd "http://www.w3.org/2001/XMLSchema#" >
    <!ENTITY skos "http://www.w3.org/2004/02/skos/core#" >
    <!ENTITY rdfs "http://www.w3.org/2000/01/rdf-schema#" >
    <!ENTITY rdf "http://www.w3.org/1999/02/22-rdf-syntax-ns#" >
    <!ENTITY bte "http://purl.org/twc/vocab/between-the-edges/" >
]>


<rdf:RDF xmlns="&bte;#"
     xml:base="http://purl.org/twc/vocab/between-the-edges/"
     xmlns:rdfs="http://www.w3.org/2000/01/rdf-schema#"
     xmlns:owl="http://www.w3.org/2002/07/owl#"
     xmlns:xsd="http://www.w3.org/2001/XMLSchema#"
     xmlns:rdf="http://www.w3.org/1999/02/22-rdf-syntax-ns#"
     xmlns:bte="http://purl.org/twc/vocab/between-the-edges/"
     xmlns:skos="http://www.w3.org/2004/02/skos/core#"
     xmlns:dcterms="http://purl.org/dc/terms/">
    <owl:Ontology rdf:about="http://purl.org/twc/vocab/between-the-edges/">
        <rdfs:comment xml:lang="en">A vocabulary to describe the implicit relationships within the literal URI.</rdfs:comment>
        <rdfs:seeAlso rdf:resource="https://github.com/timrdf/DataFAQs/wiki/BTE-Between-The-Edges"/>
    </owl:Ontology>
    


    <!-- 
    ///////////////////////////////////////////////////////////////////////////////////////
    //
    // Annotation properties
    //
    ///////////////////////////////////////////////////////////////////////////////////////
     -->

    


    <!-- http://www.w3.org/2000/01/rdf-schema#comment -->

    <owl:AnnotationProperty rdf:about="&rdfs;comment"/>
    


    <!-- 
    ///////////////////////////////////////////////////////////////////////////////////////
    //
    // Object Properties
    //
    ///////////////////////////////////////////////////////////////////////////////////////
     -->

    


    <!-- http://purl.org/twc/vocab/between-the-edges/broader -->

    <owl:ObjectProperty rdf:about="&bte;broader">
        <rdfs:domain rdf:resource="&bte;Node"/>
        <rdfs:range rdf:resource="&bte;Node"/>
    </owl:ObjectProperty>
    


    <!-- 
    ///////////////////////////////////////////////////////////////////////////////////////
    //
    // Data properties
    //
    ///////////////////////////////////////////////////////////////////////////////////////
     -->

    


    <!-- http://purl.org/twc/vocab/between-the-edges/length -->

    <owl:DatatypeProperty rdf:about="&bte;length">
        <rdfs:comment xml:lang="en">The string length of the URI.</rdfs:comment>
    </owl:DatatypeProperty>
    


    <!-- http://purl.org/twc/vocab/between-the-edges/scheme -->

    <owl:DatatypeProperty rdf:about="&bte;scheme">
        <rdfs:comment xml:lang="en">The addressing scheme of the URL. For example, http, file, gopher, mailto, ftp, etc.</rdfs:comment>
    </owl:DatatypeProperty>
    


    <!-- http://purl.org/twc/vocab/between-the-edges/step -->

    <owl:DatatypeProperty rdf:about="&bte;step">
        <rdfs:comment xml:lang="en">The local name portion of the URI, after the slash.</rdfs:comment>
    </owl:DatatypeProperty>
    


    <!-- 
    ///////////////////////////////////////////////////////////////////////////////////////
    //
    // Classes
    //
    ///////////////////////////////////////////////////////////////////////////////////////
     -->

    


    <!-- http://purl.org/twc/vocab/between-the-edges/HashEndURI -->

    <owl:Class rdf:about="&bte;HashEndURI">
        <rdfs:subClassOf rdf:resource="&bte;HashURI"/>
    </owl:Class>
    


    <!-- http://purl.org/twc/vocab/between-the-edges/HashURI -->

    <owl:Class rdf:about="&bte;HashURI">
        <rdfs:subClassOf rdf:resource="&bte;RDFNode"/>
        <rdfs:comment xml:lang="en">URI contains a hash (#). For example, &lt;http://dailymed.nlm.nih.gov/dailymed/help.cfm#webservices&gt;.</rdfs:comment>
    </owl:Class>
    


    <!-- http://purl.org/twc/vocab/between-the-edges/Node -->

    <owl:Class rdf:about="&bte;Node">
        <rdfs:comment xml:lang="en">Any rdfs:Resource that is output by a Between The Edges analysis.</rdfs:comment>
    </owl:Class>
    


    <!-- http://purl.org/twc/vocab/between-the-edges/RDFNode -->

    <owl:Class rdf:about="&bte;RDFNode">
        <rdfs:subClassOf rdf:resource="&bte;Node"/>
        <rdfs:comment xml:lang="en">An rdfs:Resource that was analyzed by Between The Edges, as opposed to rdfs:Resources that resulted from the Between The Edges analysis.</rdfs:comment>
    </owl:Class>
    


    <!-- http://purl.org/twc/vocab/between-the-edges/SlashEndURI -->

    <owl:Class rdf:about="&bte;SlashEndURI">
        <rdfs:subClassOf rdf:resource="&bte;SlashURI"/>
    </owl:Class>
    


    <!-- http://purl.org/twc/vocab/between-the-edges/SlashURI -->

    <owl:Class rdf:about="&bte;SlashURI">
        <rdfs:subClassOf rdf:resource="&bte;RDFNode"/>
    </owl:Class>

    <dcterms:FileFormat rdf:about="http://purl.org/twc/vocab/between-the-edges/PrefixTree">
        <rdfs:comment xml:lang="en">A concise tree format organizes strings by their common prefixes. Includes local and recursive weight counts.</rdfs:comment>
        <rdfs:seeAlso rdf:resource="https://github.com/timrdf/DataFAQs/wiki/BTE-Between-The-Edges#prefixtree"/>
    </dcterms:FileFormat>

</rdf:RDF>



<!-- Generated by the OWL API (version 3.4.2) http://owlapi.sourceforge.net -->

